extraction/Interop.ml
@@ -1,2 +1,9 @@
+exception NotImplemented of string
+
 let line_terminators = '\n' :: '\r' :: []
 let all_chars = List.init 128 (Char.chr)
+
+let code_point c = c
+let to_upper_case c = Char.uppercase_ascii c
+let code_points_to_string c = c :: []
+let case_fold _ = raise (NotImplemented "case_fold")
