test/Tests.ml
@@ -6,28 +6,28 @@ let%expect_test "char_class_atom_0_pos" =
   test_regex
     (CharacterClass (NoninvertedCC (ClassAtomCR ('a', EmptyCR))))
     "abbb"
-    0;
+    0 ();
   [%expect {| Matched 1 characters ([0-1]) in 'abbb' (length=4) |}]
 
 let%expect_test "char_class_atom_0_neg" =
   test_regex
     (CharacterClass (NoninvertedCC (ClassAtomCR ('b', EmptyCR))))
     "abbb"
-    0;
+    0 ();
   [%expect {| No match on 'abbb' |}]
 
 let%expect_test "negated_char_class_atom_0_pos" =
   test_regex
     (CharacterClass (InvertedCC (ClassAtomCR ('b', EmptyCR))))
     "abbb"
-    0;
+    0 ();
   [%expect {| Matched 1 characters ([0-1]) in 'abbb' (length=4) |}]
 
 let%expect_test "negated_char_class_atom_0_neg" =
   test_regex
     (CharacterClass (InvertedCC (ClassAtomCR ('a', EmptyCR))))
     "abbb"
-    0;
+    0 ();
   [%expect {| No match on 'abbb' |}]
 
 
@@ -37,35 +37,35 @@ let%expect_test "char_class_seq_0_pos_0" =
   test_regex
     (CharacterClass (NoninvertedCC (RangeCR ('a', 'c', EmptyCR))))
     "abbb"
-    0;
+    0 ();
   [%expect {| Matched 1 characters ([0-1]) in 'abbb' (length=4) |}]
 
 let%expect_test "char_class_seq_0_pos_1" =
   test_regex
     (CharacterClass (NoninvertedCC (RangeCR ('a', 'c', EmptyCR))))
     "bbbb"
-    0;
+    0 ();
   [%expect {| Matched 1 characters ([0-1]) in 'bbbb' (length=4) |}]
 
 let%expect_test "char_class_seq_0_pos_2" =
   test_regex
     (CharacterClass (NoninvertedCC (RangeCR ('a', 'c', EmptyCR))))
     "cbbb"
-    0;
+    0 ();
   [%expect {| Matched 1 characters ([0-1]) in 'cbbb' (length=4) |}]
 
 let%expect_test "char_class_seq_0_neg_0" =
   test_regex
     (CharacterClass (NoninvertedCC (RangeCR ('a', 'c', EmptyCR))))
     " bbb"
-    0;
+    0 ();
   [%expect {| No match on ' bbb' |}]
 
 let%expect_test "char_class_seq_0_neg_1" =
   test_regex
     (CharacterClass (NoninvertedCC (RangeCR ('a', 'c', EmptyCR))))
     "dbbb"
-    0;
+    0 ();
   [%expect {| No match on 'dbbb' |}]
 
 
@@ -76,35 +76,35 @@ let%expect_test "negated_char_class_seq_0_neg_0" =
   test_regex
     (CharacterClass (InvertedCC (RangeCR ('a', 'c', EmptyCR))))
     "abbb"
-    0;
+    0 ();
   [%expect {| No match on 'abbb' |}]
 
 let%expect_test "negated_char_class_seq_0_neg_1" =
   test_regex
     (CharacterClass (InvertedCC (RangeCR ('a', 'c', EmptyCR))))
     "bbbb"
-    0;
+    0 ();
   [%expect {| No match on 'bbbb' |}]
 
 let%expect_test "negated_char_class_seq_0_neg_2" =
   test_regex
     (CharacterClass (InvertedCC (RangeCR ('a', 'c', EmptyCR))))
     "cbbb"
-    0;
+    0 ();
   [%expect {| No match on 'cbbb' |}]
 
 let%expect_test "negated_char_class_seq_0_pos_0" =
   test_regex
     (CharacterClass (InvertedCC (RangeCR ('a', 'c', EmptyCR))))
     " bbb"
-    0;
+    0 ();
   [%expect {| Matched 1 characters ([0-1]) in ' bbb' (length=4) |}]
 
 let%expect_test "negated_char_class_seq_0_pos_1" =
   test_regex
     (CharacterClass (InvertedCC (RangeCR ('a', 'c', EmptyCR))))
     "dbbb"
-    0;
+    0 ();
   [%expect {|Matched 1 characters ([0-1]) in 'dbbb' (length=4) |}]
 
 
@@ -115,7 +115,7 @@ let%expect_test "sequence" =
   test_regex
     ((char 'a') -- (char 'b') -- (char 'b'))
     "abbb"
-    0;
+    0 ();
   [%expect {| Matched 3 characters ([0-3]) in 'abbb' (length=4) |}]
 
 
@@ -123,7 +123,7 @@ let%expect_test "greedy_star" =
   test_regex
     (!* (char 'a'))
     "aaaaa"
-    0;
+    0 ();
   [%expect {| Matched 5 characters ([0-5]) in 'aaaaa' (length=5) |}]
 
 
@@ -131,14 +131,14 @@ let%expect_test "lazy_star_0" =
   test_regex
     (!*? (char 'a'))
     "aaaaa"
-    0;
+    0 ();
   [%expect {| Matched 0 characters ([0-0]) in 'aaaaa' (length=5) |}]
 
 let%expect_test "lazy_star_1" = 
   test_regex
     (!*? (char 'a') -- (char 'b'))
     "aaaaab"
-    0;
+    0 ();
   [%expect {| Matched 6 characters ([0-6]) in 'aaaaab' (length=6) |}]
 
 let%expect_test "groups" =
@@ -146,7 +146,7 @@ let%expect_test "groups" =
     (   group ( char 'a')
     ||  group ( char 'b'))
     "ab"
-    0;
+    0 ();
   [%expect {|
     Matched 1 characters ([0-1]) in 'ab' (length=2)
     Group 1: 'a' ([0-1])
@@ -158,7 +158,7 @@ let%expect_test "capture_reset" =
     !*( group (char 'a')
     ||  group (char 'b'))
     "ab"
-    0;
+    0 ();
   [%expect {|
     Matched 2 characters ([0-2]) in 'ab' (length=2)
     Group 1: undefined
@@ -169,21 +169,21 @@ let%expect_test "lookahead_0_pos" =
   test_regex
     (char 'a' -- (?= (char 'b')))
     "ab"
-    0;
+    0 ();
   [%expect {| Matched 1 characters ([0-1]) in 'ab' (length=2) |}]
 
 let%expect_test "lookahead_0_neg_0" =
   test_regex
     (char 'a' -- (?= (char 'b')))
     "a"
-    0;
+    0 ();
   [%expect {| No match on 'a' |}]
 
 let%expect_test "lookahead_0_neg_1" =
   test_regex
     (char 'a' -- (?= (char 'b')))
     "aa"
-    0;
+    0 ();
   [%expect {| No match on 'aa' |}]
 
 
@@ -191,21 +191,21 @@ let%expect_test "lookbehind_0_pos" =
   test_regex
     ((?<= (char 'a')) -- char 'b')
     "ab"
-    1;
+    1 ();
   [%expect {| Matched 1 characters ([1-2]) in 'ab' (length=2) |}]
 
 let%expect_test "lookbehind_0_neg_0" =
   test_regex
     ((?<= (char 'a')) -- char 'b')
     "b"
-    0;
+    0 ();
   [%expect {| No match on 'b' |}]
 
 let%expect_test "lookbehind_0_neg_1" =
   test_regex
     ((?<= (char 'a')) -- char 'b')
     "bb"
-    1;
+    1 ();
   [%expect {| No match on 'bb' |}]
 
 
@@ -214,21 +214,21 @@ let%expect_test "neglookahead_0_pos_0" =
   test_regex
     (char 'a' -- (?! (char 'b')))
     "aa"
-    0;
+    0 ();
   [%expect {| Matched 1 characters ([0-1]) in 'aa' (length=2) |}]
 
 let%expect_test "neglookahead_0_pos_1" =
   test_regex
     (char 'a' -- (?! (char 'b')))
     "a"
-    0;
+    0 ();
   [%expect {| Matched 1 characters ([0-1]) in 'a' (length=1) |}]
 
 let%expect_test "neglookahead_0_neg" =
   test_regex
     (char 'a' -- (?! (char 'b')))
     "ab"
-    0;
+    0 ();
   [%expect {| No match on 'ab' |}]
 
 
@@ -236,28 +236,28 @@ let%expect_test "neglookbehind_0_pos_0" =
   test_regex
     ((?<! (char 'a')) -- char 'b')
     "bb"
-    1;
+    1 ();
   [%expect {| Matched 1 characters ([1-2]) in 'bb' (length=2) |}]
 
 let%expect_test "neglookbehind_0_pos_1" =
   test_regex
     ((?<! (char 'a')) -- char 'b')
     "b"
-    0;
+    0 ();
   [%expect {| Matched 1 characters ([0-1]) in 'b' (length=1) |}]
 
 let%expect_test "neglookbehind_0_neg" =
   test_regex
     ((?<! (char 'a')) -- char 'b')
     "ab"
-    1;
+    1 ();
   [%expect {| No match on 'ab' |}]
 
 let%expect_test "backref_0_pos" =
   test_regex
     (group ((char 'a')) -- !$ 1)
     "aa"
-    0;
+    0 ();
   [%expect {|
     Matched 2 characters ([0-2]) in 'aa' (length=2)
     Group 1: 'a' ([0-1]) |}]
@@ -266,21 +266,21 @@ let%expect_test "backref_0_neg_0" =
   test_regex
     (group ((char 'a')) -- !$ 1)
     "ab"
-    0;
+    0 ();
   [%expect {| No match on 'ab' |}]
 
 let%expect_test "backref_0_neg_1" =
   test_regex
     (group ((char 'a')) -- !$ 1)
     "a"
-    0;
+    0 ();
   [%expect {| No match on 'a' |}]
 
 let%expect_test "backref_undefined" =
   test_regex
     ((group ((char 'a')) || group ((char 'b'))) -- !$ 2)
     "aa"
-    0;
+    0 ();
   [%expect {|
     Matched 1 characters ([0-1]) in 'aa' (length=2)
     Group 1: 'a' ([0-1])
@@ -290,7 +290,7 @@ let%expect_test "backref_multiple" =
   test_regex
     (group ((char 'a')) -- !$ 1 -- !$ 2 -- group ((char 'b')) -- !$ 1 -- !$ 2)
     "aabab"
-    0;
+    0 ();
   [%expect {|
     Matched 5 characters ([0-5]) in 'aabab' (length=5)
     Group 1: 'a' ([0-1])
@@ -300,7 +300,7 @@ let%expect_test "backref_long_pos" =
   test_regex
     (group ((char 'a') -- (char 'b') -- (char 'a')) -- !$ 1)
     "abaaba"
-    0;
+    0 ();
   [%expect {|
     Matched 6 characters ([0-6]) in 'abaaba' (length=6)
     Group 1: 'aba' ([0-3]) |}]
@@ -309,26 +309,74 @@ let%expect_test "backref_long_neg_0" =
   test_regex
     (group ((char 'a') -- (char 'b') -- (char 'a')) -- !$ 1)
     "abaab"
-    0;
+    0 ();
   [%expect {| No match on 'abaab' |}]
 
 let%expect_test "backref_long_neg_1" =
 test_regex
   (group ((char 'a') -- (char 'b') -- (char 'a')) -- !$ 1)
   "abacba"
-  0;
+  0 ();
 [%expect {| No match on 'abacba' |}]
 
 let%expect_test "backref_long_neg_2" =
   test_regex
     (group ((char 'a') -- (char 'b') -- (char 'a')) -- !$ 1)
     "abaaca"
-    0;
+    0 ();
   [%expect {| No match on 'abaaca' |}]
 
 let%expect_test "backref_long_neg_3" =
   test_regex
     (group ((char 'a') -- (char 'b') -- (char 'a')) -- !$ 1)
     "abaabc"
-    0;
+    0 ();
   [%expect {| No match on 'abaabc' |}]
+
+
+
+
+
+
+let%expect_test "case_insensitive_0_pos_0" =
+  test_regex
+    (CharacterClass (NoninvertedCC (ClassAtomCR ('a', EmptyCR))))
+    "abbb"
+    0 ~ignoreCase:true ();
+  [%expect {| Matched 1 characters ([0-1]) in 'abbb' (length=4) |}]
+
+let%expect_test "case_insensitive_0_pos_1" =
+  test_regex
+    (CharacterClass (NoninvertedCC (ClassAtomCR ('a', EmptyCR))))
+    "Abbb"
+    0 ~ignoreCase:true ();
+  [%expect {| Matched 1 characters ([0-1]) in 'Abbb' (length=4) |}]
+
+let%expect_test "case_insensitive_0_pos_2" =
+  test_regex
+    (CharacterClass (NoninvertedCC (ClassAtomCR ('A', EmptyCR))))
+    "abbb"
+    0 ~ignoreCase:true ();
+  [%expect {| Matched 1 characters ([0-1]) in 'abbb' (length=4) |}]
+
+let%expect_test "case_insensitive_0_pos_3" =
+  test_regex
+    (CharacterClass (NoninvertedCC (ClassAtomCR ('A', EmptyCR))))
+    "Abbb"
+    0 ~ignoreCase:true ();
+  [%expect {| Matched 1 characters ([0-1]) in 'Abbb' (length=4) |}]
+
+
+let%expect_test "case_insensitive_0_neg_0" =
+  test_regex
+    (CharacterClass (NoninvertedCC (ClassAtomCR ('a', EmptyCR))))
+    "bbbb"
+    0 ~ignoreCase:true ();
+  [%expect {| No match on 'bbbb' |}]
+
+let%expect_test "case_insensitive_0_neg_1" =
+  test_regex
+    (CharacterClass (NoninvertedCC (ClassAtomCR ('a', EmptyCR))))
+    "Bbbb"
+    0 ~ignoreCase:true ();
+  [%expect {| No match on 'Bbbb' |}]
