MECMAR/props/Correctness.v
@@ -9,6 +9,25 @@ Module Correctness.
   Import Notation.
   Import Semantics.
 
+  Lemma canonicalize_success: forall rer a, exists v, canonicalize rer a = Success v.
+  Proof.
+    intros. remember (canonicalize rer a) as r eqn:C. unfold canonicalize in C.
+    focus § _ _ [] § auto destruct in C; try solve [ focus § _ _ (_ []) § do (fun v => exists v) in C; subst; reflexivity ].
+    - hypotheses_reflector. spec_reflector Nat.eqb_spec. apply List.Unique.failure_bounds in AutoDest_2. easy.
+  Qed.
+
+  Ltac rewrite_canonicalize := repeat lazymatch goal with 
+        | [ H: context[ canonicalize ?rer ?c ] |- _ ] =>
+            lazymatch goal with
+            | [ _: canonicalize rer c = Success _ |- _ ] => idtac
+            | [ |- _ ] =>
+                let d := fresh "canonicalized_" c in
+                let Eq := fresh "Eq_" d in
+                pose proof (canonicalize_success rer c) as [ d Eq ];
+                rewrite -> Eq in *
+            end
+        end.
+
   Create HintDb Warblre.
   #[export] Hint Unfold repeatMatcherFuel wrap_option : Warblre.
 
@@ -724,9 +743,9 @@ Module Correctness.
       - search.
         + Zhelper. MatchState.solve_with lia.
         + apply Progress.step. lia.
-      - injection Eq_oof as <-. apply List.Exists.failure_kind in AutoDest_1.
-        destruct AutoDest_1 as [ i [ v [ Indexed_A_i Eq_v_s ]]].
-        discriminate.
+      - injection Eq_oof as <-. unfold CharSet.exist in AutoDest_2. apply List.Exists.failure_kind in AutoDest_2 as [_ [ c' [ _ Can_failure ]]].
+        rewrite_canonicalize. discriminate.
+      - rewrite_canonicalize. discriminate.
       - injection Eq_oof as ->. boolean_simplifier. Zhelper.
         destruct Vx as [ Eq_str [ [ ? ? ] _ ]].
         destruct dir.
@@ -788,12 +807,31 @@ Module Correctness.
         rename s into t_s, e into t_e, H into Ineq_t, H0 into IO_t_s, H1 into IO_t_e.
         MatchState.normalize. cbn in *. rewrite -> List.Range.Int.Bounds.length in *.
         focus § _ [] _ § auto destruct in Eq_af; injection Eq_af as ->.
+        + rewrite_canonicalize. discriminate.
+        + destruct dir.
+          * apply List.Indexing.Int.failure_bounds in AutoDest_2 as [ ? | ? ]; lia.
+          * apply List.Indexing.Int.failure_bounds in AutoDest_2 as [ ? | ? ]; lia.
+        + rewrite_canonicalize. discriminate.
+        + destruct dir.
+          * apply List.Indexing.Int.failure_bounds in AutoDest_0 as [ ? | ? ]; lia.
+          * apply List.Indexing.Int.failure_bounds in AutoDest_0 as [ ? | ? ]; lia.
+      (* - injection Eq_af as ->. Zhelper.
+        apply List.Exists.failure_kind in AutoDest_3.
+        destruct AutoDest_3 as [ i [ j [ Eq_indexed Eq_af ]]].
+        pose proof Eq_indexed as Tmp. apply List.Range.Int.Bounds.indexing in Tmp as ->.
+        apply List.Indexing.Int.success_bounds in Eq_indexed as Bounds_i. clear Eq_indexed.
+        destruct Vx as [ Eq_str [ [ ? ? ] [ _ V_t ]]].
+        cbn in AutoDest_. focus § _ [] _ § auto destruct in AutoDest_.
+        specialize (V_t _ _ AutoDest_). dependent destruction V_t.
+        rename s into t_s, e into t_e, H into Ineq_t, H0 into IO_t_s, H1 into IO_t_e.
+        MatchState.normalize. cbn in *. rewrite -> List.Range.Int.Bounds.length in *.
+        focus § _ [] _ § auto destruct in Eq_af; injection Eq_af as ->.
         + destruct dir.
           * apply List.Indexing.Int.failure_bounds in AutoDest_1 as [ ? | ? ]; lia.
           * apply List.Indexing.Int.failure_bounds in AutoDest_1 as [ ? | ? ]; lia.
         + destruct dir.
           * apply List.Indexing.Int.failure_bounds in AutoDest_0 as [ ? | ? ]; lia.
-          * apply List.Indexing.Int.failure_bounds in AutoDest_0 as [ ? | ? ]; lia.
+          * apply List.Indexing.Int.failure_bounds in AutoDest_0 as [ ? | ? ]; lia. *)
       - injection Eq_af as ->.
         cbn in AutoDest_. focus § _ [] _ § auto destruct in AutoDest_.
         apply List.Indexing.Nat.failure_bounds in AutoDest_.
@@ -1073,9 +1111,10 @@ Module Correctness.
       - search.
         + Zhelper. MatchState.solve_with lia.
         + apply Progress.step. lia.
-      - injection Eq_oof as ->. apply List.Exists.failure_kind in AutoDest_1.
-        destruct AutoDest_1 as [ i [ v [ Indexed_A_i Eq_v_s ]]].
-        discriminate.
+      - injection Eq_oof as ->.
+        unfold CharSet.exist in AutoDest_2. apply List.Exists.failure_kind in AutoDest_2 as [ i [ v [ ? ? ]]].
+        rewrite_canonicalize. discriminate.
+      - injection Eq_oof as ->. rewrite_canonicalize. discriminate.
       - injection Eq_oof as ->.
         pose proof (@List.Indexing.Int.failure_kind Character) as Falsum. specialize Falsum  with (1 := AutoDest_0).
         cbn in *. congruence.
@@ -1121,12 +1160,12 @@ Module Correctness.
       - injection Eq_oof as ->.
         apply List.Exists.failure_kind in AutoDest_3.
         destruct AutoDest_3 as [ i [ j [ Eq_indexed Eq_oof ]]].
-        focus § _ [] _ § auto destruct in Eq_oof.
-        + injection Eq_oof as ->.
-          pose proof (@List.Indexing.Int.failure_kind Character) as Falsum. specialize Falsum  with (1 := AutoDest_4).
+        focus § _ [] _ § auto destruct in Eq_oof; injection Eq_oof as ->.
+        + rewrite_canonicalize. discriminate.
+        + pose proof (@List.Indexing.Int.failure_kind Character) as Falsum. specialize Falsum  with (1 := AutoDest_5).
           cbn in *. congruence.
-        + injection Eq_oof as ->.
-          pose proof (@List.Indexing.Int.failure_kind Character) as Falsum. specialize Falsum  with (1 := AutoDest_3).
+        + rewrite_canonicalize. discriminate.
+        + pose proof (@List.Indexing.Int.failure_kind Character) as Falsum. specialize Falsum  with (1 := AutoDest_3).
           cbn in *. congruence.
       - injection Eq_oof as ->.
         pose proof @List.Indexing.Nat.failure_kind as Falsum.
